wip: lib

lib/Lib.IntVector.Transpose.fst
@@ -3,13 +3,13 @@ module Lib.IntVector.Transpose
 module Loops = Lib.LoopCombinators
 
 
-#set-options "--z3rlimit 50 --max_fuel 0 --max_ifuel 0"
+#set-options "--z3rlimit 50 --fuel 0 --ifuel 0"
 
 ///
 ///  transpose4x4
 ///
 
-inline_for_extraction noextract
+inline_for_extraction
 val transpose4x4_0: #t:v_inttype -> vec_t4 t -> vec_t4 t
 let transpose4x4_0 #t (v0,v1,v2,v3) =
   let v0' = vec_interleave_low v0 v1 in
@@ -24,7 +24,7 @@ let transpose4x4_0 #t (v0,v1,v2,v3) =
   (v0'',v2'',v1'',v3'')
 
 
-inline_for_extraction noextract
+inline_for_extraction
 val transpose4x4_uint32: #t:v_inttype{t == U32} -> vec_t4 t -> vec_t4 t
 let transpose4x4_uint32 #t vs =
   [@inline_let]
@@ -32,7 +32,7 @@ let transpose4x4_uint32 #t vs =
   (v0'',v1'',v2'',v3'')
 
 
-inline_for_extraction noextract
+inline_for_extraction
 val transpose4x4_uint64: #t:v_inttype{t == U64} -> vec_t4 t -> vec_t4 t
 let transpose4x4_uint64 #t vs = transpose4x4_0 #t vs
 
@@ -46,7 +46,7 @@ let transpose4x4 #t vs =
 ///   transpose8x8
 ///
 
-inline_for_extraction noextract
+inline_for_extraction
 val transpose8x8_0: #t:v_inttype -> vec_t8 t -> vec_t8 t
 let transpose8x8_0 #t (v0,v1,v2,v3,v4,v5,v6,v7) =
   let v0' = vec_interleave_low v0 v1 in
@@ -60,7 +60,7 @@ let transpose8x8_0 #t (v0,v1,v2,v3,v4,v5,v6,v7) =
   (v0',v1',v2',v3',v4',v5',v6',v7')
 
 
-inline_for_extraction noextract
+inline_for_extraction
 val transpose8x8_1: #t:v_inttype -> vec_t8 t -> vec_t8 t
 let transpose8x8_1 #t (v0,v1,v2,v3,v4,v5,v6,v7) =
   let v0' = vec_interleave_low_n 2 v0 v2 in
@@ -74,7 +74,7 @@ let transpose8x8_1 #t (v0,v1,v2,v3,v4,v5,v6,v7) =
   (v0',v1',v2',v3',v4',v5',v6',v7')
 
 
-inline_for_extraction noextract
+inline_for_extraction
 val transpose8x8_2: #t:v_inttype -> vec_t8 t -> vec_t8 t
 let transpose8x8_2 #t (v0,v1,v2,v3,v4,v5,v6,v7) =
   let v0' = vec_interleave_low_n 4 v0 v4 in
@@ -88,7 +88,7 @@ let transpose8x8_2 #t (v0,v1,v2,v3,v4,v5,v6,v7) =
   (v0',v1',v2',v3',v4',v5',v6',v7')
 
 
-inline_for_extraction noextract
+inline_for_extraction
 val transpose8x8_012: #t:v_inttype -> vec_t8 t -> vec_t8 t
 let transpose8x8_012 #t vs0 =
   let (v0,v1,v2,v3,v4,v5,v6,v7) = vs0 in
@@ -101,7 +101,7 @@ let transpose8x8_012 #t vs0 =
   (v0',v1',v2',v3',v4',v5',v6',v7')
 
 
-inline_for_extraction noextract
+inline_for_extraction
 val transpose8x8_uint32: #t:v_inttype{t == U32} -> vec_t8 t -> vec_t8 t
 let transpose8x8_uint32 #t vs0 =
   [@inline_let]
@@ -109,146 +109,9 @@ let transpose8x8_uint32 #t vs0 =
   (v0',v2',v1',v3',v4',v6',v5',v7')
 
 
-inline_for_extraction noextract
-val transpose8x8_uint64: #t:v_inttype{t == U64} -> vec_t8 t -> vec_t8 t
-let transpose8x8_uint64 #t vs0 =
-  transpose8x8_012 #t vs0
-
-
 let transpose8x8 #t vs =
   match t with
   | U32 -> transpose8x8_uint32 #t vs
-  | U64 -> transpose8x8_uint64 #t vs
-
-///
-///  transpose16x16
-///
-
-inline_for_extraction noextract
-val transpose16x16_uint32_0: #t:v_inttype{t == U32} -> vs:(vec_t16 t & vec_t16 t) -> (vec_t16 t & vec_t16 t)
-let transpose16x16_uint32_0 #t vs =
-  let ((v0,v1,v2,v3,v4,v5,v6,v7),(v8,v9,v10,v11,v12,v13,v14,v15)) = vs in
-
-  let v0' = vec_interleave_low v0 v1 in
-  let v1' = vec_interleave_high v0 v1 in
-  let v2' = vec_interleave_low v2 v3 in
-  let v3' = vec_interleave_high v2 v3 in
-  let v4' = vec_interleave_low v4 v5 in
-  let v5' = vec_interleave_high v4 v5 in
-  let v6' = vec_interleave_low v6 v7 in
-  let v7' = vec_interleave_high v6 v7 in
-  let v8' = vec_interleave_low v8 v9 in
-  let v9' = vec_interleave_high v8 v9 in
-  let v10' = vec_interleave_low v10 v11 in
-  let v11' = vec_interleave_high v10 v11 in
-  let v12' = vec_interleave_low v12 v13 in
-  let v13' = vec_interleave_high v12 v13 in
-  let v14' = vec_interleave_low v14 v15 in
-  let v15' = vec_interleave_high v14 v15 in
-
-  ((v0',v1',v2',v3',v4',v5',v6',v7'),(v8',v9',v10',v11',v12',v13',v14',v15'))
-
-
-inline_for_extraction noextract
-val transpose16x16_uint32_1: #t:v_inttype{t == U32} -> vs:(vec_t16 t & vec_t16 t) -> (vec_t16 t & vec_t16 t)
-let transpose16x16_uint32_1 #t vs =
-  let ((v0,v1,v2,v3,v4,v5,v6,v7),(v8,v9,v10,v11,v12,v13,v14,v15)) = vs in
-
-  let v0' = vec_interleave_low_n 2 v0 v2 in
-  let v2' = vec_interleave_high_n 2 v0 v2 in
-  let v1' = vec_interleave_low_n 2 v1 v3 in
-  let v3' = vec_interleave_high_n 2 v1 v3 in
-  let v4' = vec_interleave_low_n 2 v4 v6 in
-  let v6' = vec_interleave_high_n 2 v4 v6 in
-  let v5' = vec_interleave_low_n 2 v5 v7 in
-  let v7' = vec_interleave_high_n 2 v5 v7 in
-  let v8' = vec_interleave_low_n 2 v8 v10 in
-  let v10' = vec_interleave_high_n 2 v8 v10 in
-  let v9' = vec_interleave_low_n 2 v9 v11 in
-  let v11' = vec_interleave_high_n 2 v9 v11 in
-  let v12' = vec_interleave_low_n 2 v12 v14 in
-  let v14' = vec_interleave_high_n 2 v12 v14 in
-  let v13' = vec_interleave_low_n 2 v13 v15 in
-  let v15' = vec_interleave_high_n 2 v13 v15 in
-
-  ((v0',v1',v2',v3',v4',v5',v6',v7'),(v8',v9',v10',v11',v12',v13',v14',v15'))
-
-
-inline_for_extraction noextract
-val transpose16x16_uint32_2: #t:v_inttype{t == U32} -> vs:(vec_t16 t & vec_t16 t) -> (vec_t16 t & vec_t16 t)
-let transpose16x16_uint32_2 #t vs =
-  let ((v0,v1,v2,v3,v4,v5,v6,v7),(v8,v9,v10,v11,v12,v13,v14,v15)) = vs in
-
-  let v0' = vec_interleave_low_n 4 v0 v4 in
-  let v4' = vec_interleave_high_n 4 v0 v4 in
-  let v1' = vec_interleave_low_n 4 v1 v5 in
-  let v5' = vec_interleave_high_n 4 v1 v5 in
-  let v2' = vec_interleave_low_n 4 v2 v6 in
-  let v6' = vec_interleave_high_n 4 v2 v6 in
-  let v3' = vec_interleave_low_n 4 v3 v7 in
-  let v7' = vec_interleave_high_n 4 v3 v7 in
-  let v8' = vec_interleave_low_n 4 v8 v12 in
-  let v12' = vec_interleave_high_n 4 v8 v12 in
-  let v9' = vec_interleave_low_n 4 v9 v13 in
-  let v13' = vec_interleave_high_n 4 v9 v13 in
-  let v10' = vec_interleave_low_n 4 v10 v14 in
-  let v14' = vec_interleave_high_n 4 v10 v14 in
-  let v11' = vec_interleave_low_n 4 v11 v15 in
-  let v15' = vec_interleave_high_n 4 v11 v15 in
-
-  ((v0',v1',v2',v3',v4',v5',v6',v7'),(v8',v9',v10',v11',v12',v13',v14',v15'))
-
-
-inline_for_extraction noextract
-val transpose16x16_uint32_3: #t:v_inttype{t == U32} -> vs:(vec_t16 t & vec_t16 t) -> (vec_t16 t & vec_t16 t)
-let transpose16x16_uint32_3 #t vs =
-  let ((v0,v1,v2,v3,v4,v5,v6,v7),(v8,v9,v10,v11,v12,v13,v14,v15)) = vs in
-
-  let v0' = vec_interleave_low_n 8 v0 v8 in
-  let v8' = vec_interleave_high_n 8 v0 v8 in
-  let v1' = vec_interleave_low_n 8 v1 v9 in
-  let v9' = vec_interleave_high_n 8 v1 v9 in
-  let v2' = vec_interleave_low_n 8 v2 v10 in
-  let v10' = vec_interleave_high_n 8 v2 v10 in
-  let v3' = vec_interleave_low_n 8 v3 v11 in
-  let v11' = vec_interleave_high_n 8 v3 v11 in
-  let v4' = vec_interleave_low_n 8 v4 v12 in
-  let v12' = vec_interleave_high_n 8 v4 v12 in
-  let v5' = vec_interleave_low_n 8 v5 v13 in
-  let v13' = vec_interleave_high_n 8 v5 v13 in
-  let v6' = vec_interleave_low_n 8 v6 v14 in
-  let v14' = vec_interleave_high_n 8 v6 v14 in
-  let v7' = vec_interleave_low_n 8 v7 v15 in
-  let v15' = vec_interleave_high_n 8 v7 v15 in
-
-  ((v0',v1',v2',v3',v4',v5',v6',v7'),(v8',v9',v10',v11',v12',v13',v14',v15'))
-
-
-inline_for_extraction noextract
-val transpose16x16_uint32: #t:v_inttype{t == U32} -> vs:(vec_t16 t & vec_t16 t) -> (vec_t16 t & vec_t16 t)
-let transpose16x16_uint32 #t vs =
-  let ((v0,v1,v2,v3,v4,v5,v6,v7),(v8,v9,v10,v11,v12,v13,v14,v15)) = vs in
-
-  [@inline_let]
-  let ((v0',v1',v2',v3',v4',v5',v6',v7'),(v8',v9',v10',v11',v12',v13',v14',v15')) =
-    transpose16x16_uint32_0 ((v0,v1,v2,v3,v4,v5,v6,v7),(v8,v9,v10,v11,v12,v13,v14,v15)) in
-  [@inline_let]
-  let ((v0',v1',v2',v3',v4',v5',v6',v7'),(v8',v9',v10',v11',v12',v13',v14',v15')) =
-    transpose16x16_uint32_1 ((v0',v1',v2',v3',v4',v5',v6',v7'),(v8',v9',v10',v11',v12',v13',v14',v15')) in
-  [@inline_let]
-  let ((v0',v1',v2',v3',v4',v5',v6',v7'),(v8',v9',v10',v11',v12',v13',v14',v15')) =
-    transpose16x16_uint32_2 ((v0',v1',v2',v3',v4',v5',v6',v7'),(v8',v9',v10',v11',v12',v13',v14',v15')) in
-  [@inline_let]
-  let ((v0',v1',v2',v3',v4',v5',v6',v7'),(v8',v9',v10',v11',v12',v13',v14',v15')) =
-    transpose16x16_uint32_3 ((v0',v1',v2',v3',v4',v5',v6',v7'),(v8',v9',v10',v11',v12',v13',v14',v15')) in
-
-  ((v0',v2',v1',v3',v4',v6',v5',v7'),(v8',v10',v9',v11',v12',v14',v13',v15'))
-
-
-let transpose16x16 #t vs =
-  match t with
-  | U32 -> transpose16x16_uint32 #t vs
-
 
 ///
 ///  generic transpose
@@ -280,7 +143,7 @@ let lemma_l_plus_pow2i_lt #w n i l =
   }
 
 
-inline_for_extraction noextract
+inline_for_extraction
 val transposewxw_f_l:
     #w:width
   -> #t:v_inttype
@@ -300,7 +163,7 @@ let transposewxw_f_l #w #t n i vs l =
     vec_interleave_high_n (pow2 i) vs.[l - pow2 i] vs.[l]
 
 
-inline_for_extraction noextract
+inline_for_extraction
 val transposewxw_f: #w:width -> #t:v_inttype -> n:nat{pow2 n == w} -> i:nat{i < n} -> lseq (vec_t t w) w -> lseq (vec_t t w) w
 let transposewxw_f #w #t n i vs =
   createi w (transposewxw_f_l #w n i vs)
@@ -313,7 +176,7 @@ let transposewxw_lseq #w #t n vs =
 ///  transposewxw_lseq lemmas
 ///
 
-inline_for_extraction noextract
+inline_for_extraction
 let f_lseq4 (#t:v_inttype) (vs:lseq (vec_t t 4) 4) (f:vec_t4 t -> vec_t4 t) : lseq (vec_t t 4) 4 =
   let (v0,v1,v2,v3) = (vs.[0],vs.[1],vs.[2],vs.[3]) in
   let (r0,r1,r2,r3) = f (v0,v1,v2,v3) in
@@ -330,7 +193,7 @@ let transpose4x4_lseq_is_transposewxw #t vs0 =
   eq_intro (transposewxw_lseq 2 vs0) (f_lseq4 vs0 transpose4x4_0)
 
 
-inline_for_extraction noextract
+inline_for_extraction
 let f_lseq8 (#t:v_inttype) (vs:lseq (vec_t t 8) 8) (f:vec_t8 t -> vec_t8 t) : lseq (vec_t t 8) 8 =
   let (v0,v1,v2,v3,v4,v5,v6,v7) = (vs.[0],vs.[1],vs.[2],vs.[3],vs.[4],vs.[5],vs.[6],vs.[7]) in
   let (r0,r1,r2,r3,r4,r5,r6,r7) = f (v0,v1,v2,v3,v4,v5,v6,v7) in
@@ -354,46 +217,6 @@ let transpose8x8_lseq_is_transposewxw #t vs0 =
   let res2 = transposewxw_f n 2 res1 in
   eq_intro res2 (f_lseq8 res1 transpose8x8_2);
   eq_intro (transposewxw_lseq 3 vs0) (f_lseq8 vs0 transpose8x8_012)
-
-
-inline_for_extraction noextract
-let f_lseq16 (#t:v_inttype) (vs:lseq (vec_t t 16) 16)
-  (f:(vec_t16 t & vec_t16 t -> vec_t16 t & vec_t16 t)) : lseq (vec_t t 16) 16
- =
-  let (v0,v1,v2,v3,v4,v5,v6,v7) = (vs.[0],vs.[1],vs.[2],vs.[3],vs.[4],vs.[5],vs.[6],vs.[7]) in
-  let (v8,v9,v10,v11,v12,v13,v14,v15) = (vs.[8],vs.[9],vs.[10],vs.[11],vs.[12],vs.[13],vs.[14],vs.[15]) in
-  let ((r0,r1,r2,r3,r4,r5,r6,r7),(r8,r9,r10,r11,r12,r13,r14,r15)) =
-    f ((v0,v1,v2,v3,v4,v5,v6,v7), (v8,v9,v10,v11,v12,v13,v14,v15)) in
-  create16 r0 r1 r2 r3 r4 r5 r6 r7 r8 r9 r10 r11 r12 r13 r14 r15
-
-
-#push-options "--z3rlimit 100"
-val transpose16x16_lseq_is_transposewxw_uint32: vs:lseq (vec_t U32 16) 16 ->
-  Lemma
-   (let r = transposewxw_lseq 4 vs in
-    create16 r.[0] r.[2] r.[1] r.[3] r.[4] r.[6] r.[5] r.[7] r.[8] r.[10] r.[9] r.[11] r.[12] r.[14] r.[13] r.[15]
-      `Seq.equal` transpose16x16_lseq #U32 vs)
-
-let transpose16x16_lseq_is_transposewxw_uint32 vs0 =
-  let n = 4 in
-  Loops.unfold_repeati n (transposewxw_f #16 n) vs0 3;
-  Loops.unfold_repeati n (transposewxw_f #16 n) vs0 2;
-  Loops.unfold_repeati n (transposewxw_f #16 n) vs0 1;
-  Loops.unfold_repeati n (transposewxw_f #16 n) vs0 0;
-  Loops.eq_repeati0 n (transposewxw_f #16 n) vs0;
-  let r = transposewxw_lseq n vs0 in
-
-  let res0 = transposewxw_f n 0 vs0 in
-  eq_intro res0 (f_lseq16 vs0 transpose16x16_uint32_0);
-  let res1 = transposewxw_f n 1 res0 in
-  eq_intro res1 (f_lseq16 res0 transpose16x16_uint32_1);
-  let res2 = transposewxw_f n 2 res1 in
-  eq_intro res2 (f_lseq16 res1 transpose16x16_uint32_2);
-  let res3 = transposewxw_f n 3 res2 in
-  eq_intro res3 (f_lseq16 res2 transpose16x16_uint32_3);
-  let res = create16 r.[0] r.[2] r.[1] r.[3] r.[4] r.[6] r.[5] r.[7] r.[8] r.[10] r.[9] r.[11] r.[12] r.[14] r.[13] r.[15] in
-  eq_intro res (f_lseq16 vs0 transpose16x16_uint32)
-#pop-options
 
 
 val transpose4x4_lemma_uint32_ij: vs:lseq (vec_t U32 4) 4 -> i:nat{i < 4} -> j:nat{j < 4} ->
@@ -489,141 +312,6 @@ let transpose8x8_lemma_uint32_ij vs0 i j =
   vec_interleave_high_lemma_uint32_8 vs0.[6] vs0.[7]
 
 
-val transpose8x8_lemma_uint64_ij: vs:lseq (vec_t U64 8) 8 -> i:nat{i < 8} -> j:nat{j < 8} ->
-  Lemma ((vec_v (transpose8x8_lseq #U64 vs).[i]).[j] == (vec_v vs.[j]).[i])
-
-let transpose8x8_lemma_uint64_ij vs0 i j =
-  transpose8x8_lseq_is_transposewxw vs0;
-  let n = 3 in
-  Loops.unfold_repeati n (transposewxw_f #8 n) vs0 2;
-  Loops.unfold_repeati n (transposewxw_f #8 n) vs0 1;
-  Loops.unfold_repeati n (transposewxw_f #8 n) vs0 0;
-  Loops.eq_repeati0 n (transposewxw_f #8 n) vs0;
-
-  let res0 = transposewxw_f n 0 vs0 in
-  let res1 = transposewxw_f n 1 res0 in
-  let res2 = transposewxw_f n 2 res1 in
-
-  vec_interleave_low_n_lemma_uint64_8_4 res1.[0] res1.[4];
-  vec_interleave_low_n_lemma_uint64_8_4 res1.[1] res1.[5];
-  vec_interleave_low_n_lemma_uint64_8_4 res1.[2] res1.[6];
-  vec_interleave_low_n_lemma_uint64_8_4 res1.[3] res1.[7];
-  vec_interleave_high_n_lemma_uint64_8_4 res1.[0] res1.[4];
-  vec_interleave_high_n_lemma_uint64_8_4 res1.[1] res1.[5];
-  vec_interleave_high_n_lemma_uint64_8_4 res1.[2] res1.[6];
-  vec_interleave_high_n_lemma_uint64_8_4 res1.[3] res1.[7];
-
-  vec_interleave_low_n_lemma_uint64_8_2 res0.[0] res0.[2];
-  vec_interleave_low_n_lemma_uint64_8_2 res0.[1] res0.[3];
-  vec_interleave_low_n_lemma_uint64_8_2 res0.[4] res0.[6];
-  vec_interleave_low_n_lemma_uint64_8_2 res0.[5] res0.[7];
-  vec_interleave_high_n_lemma_uint64_8_2 res0.[0] res0.[2];
-  vec_interleave_high_n_lemma_uint64_8_2 res0.[1] res0.[3];
-  vec_interleave_high_n_lemma_uint64_8_2 res0.[4] res0.[6];
-  vec_interleave_high_n_lemma_uint64_8_2 res0.[5] res0.[7];
-
-  vec_interleave_low_lemma_uint64_8 vs0.[0] vs0.[1];
-  vec_interleave_low_lemma_uint64_8 vs0.[2] vs0.[3];
-  vec_interleave_low_lemma_uint64_8 vs0.[4] vs0.[5];
-  vec_interleave_low_lemma_uint64_8 vs0.[6] vs0.[7];
-  vec_interleave_high_lemma_uint64_8 vs0.[0] vs0.[1];
-  vec_interleave_high_lemma_uint64_8 vs0.[2] vs0.[3];
-  vec_interleave_high_lemma_uint64_8 vs0.[4] vs0.[5];
-  vec_interleave_high_lemma_uint64_8 vs0.[6] vs0.[7]
-
-
-#push-options "--z3rlimit 200"
-val transpose16x16_lemma_ij: vs:lseq (vec_t U32 16) 16 -> i:nat{i < 16} -> j:nat{j < 16} ->
-  Lemma ((vec_v (transpose16x16_lseq #U32 vs).[i]).[j] == (vec_v vs.[j]).[i])
-
-let transpose16x16_lemma_ij vs0 i j =
-  transpose16x16_lseq_is_transposewxw_uint32 vs0;
-
-  Loops.unfold_repeati 4 (transposewxw_f 4) vs0 3;
-  Loops.unfold_repeati 4 (transposewxw_f 4) vs0 2;
-  Loops.unfold_repeati 4 (transposewxw_f 4) vs0 1;
-  Loops.unfold_repeati 4 (transposewxw_f 4) vs0 0;
-  Loops.eq_repeati0 4 (transposewxw_f 4) vs0;
-
-  let res0 = transposewxw_f 4 0 vs0 in
-  let res1 = transposewxw_f 4 1 res0 in
-  let res2 = transposewxw_f 4 2 res1 in
-  let res3 = transposewxw_f 4 3 res2 in
-
-  vec_interleave_low_n_lemma_uint32_16_8 res2.[0] res2.[8];
-  vec_interleave_low_n_lemma_uint32_16_8 res2.[1] res2.[9];
-  vec_interleave_low_n_lemma_uint32_16_8 res2.[2] res2.[10];
-  vec_interleave_low_n_lemma_uint32_16_8 res2.[3] res2.[11];
-  vec_interleave_low_n_lemma_uint32_16_8 res2.[4] res2.[12];
-  vec_interleave_low_n_lemma_uint32_16_8 res2.[5] res2.[13];
-  vec_interleave_low_n_lemma_uint32_16_8 res2.[6] res2.[14];
-  vec_interleave_low_n_lemma_uint32_16_8 res2.[7] res2.[15];
-
-  vec_interleave_high_n_lemma_uint32_16_8 res2.[0] res2.[8];
-  vec_interleave_high_n_lemma_uint32_16_8 res2.[1] res2.[9];
-  vec_interleave_high_n_lemma_uint32_16_8 res2.[2] res2.[10];
-  vec_interleave_high_n_lemma_uint32_16_8 res2.[3] res2.[11];
-  vec_interleave_high_n_lemma_uint32_16_8 res2.[4] res2.[12];
-  vec_interleave_high_n_lemma_uint32_16_8 res2.[5] res2.[13];
-  vec_interleave_high_n_lemma_uint32_16_8 res2.[6] res2.[14];
-  vec_interleave_high_n_lemma_uint32_16_8 res2.[7] res2.[15];
-
-  vec_interleave_low_n_lemma_uint32_16_4 res1.[0] res1.[4];
-  vec_interleave_low_n_lemma_uint32_16_4 res1.[1] res1.[5];
-  vec_interleave_low_n_lemma_uint32_16_4 res1.[2] res1.[6];
-  vec_interleave_low_n_lemma_uint32_16_4 res1.[3] res1.[7];
-  vec_interleave_low_n_lemma_uint32_16_4 res1.[8] res1.[12];
-  vec_interleave_low_n_lemma_uint32_16_4 res1.[9] res1.[13];
-  vec_interleave_low_n_lemma_uint32_16_4 res1.[10] res1.[14];
-  vec_interleave_low_n_lemma_uint32_16_4 res1.[11] res1.[15];
-
-  vec_interleave_high_n_lemma_uint32_16_4 res1.[0] res1.[4];
-  vec_interleave_high_n_lemma_uint32_16_4 res1.[1] res1.[5];
-  vec_interleave_high_n_lemma_uint32_16_4 res1.[2] res1.[6];
-  vec_interleave_high_n_lemma_uint32_16_4 res1.[3] res1.[7];
-  vec_interleave_high_n_lemma_uint32_16_4 res1.[8] res1.[12];
-  vec_interleave_high_n_lemma_uint32_16_4 res1.[9] res1.[13];
-  vec_interleave_high_n_lemma_uint32_16_4 res1.[10] res1.[14];
-  vec_interleave_high_n_lemma_uint32_16_4 res1.[11] res1.[15];
-
-  vec_interleave_low_n_lemma_uint32_16_2 res0.[0] res0.[2];
-  vec_interleave_low_n_lemma_uint32_16_2 res0.[1] res0.[3];
-  vec_interleave_low_n_lemma_uint32_16_2 res0.[4] res0.[6];
-  vec_interleave_low_n_lemma_uint32_16_2 res0.[5] res0.[7];
-  vec_interleave_low_n_lemma_uint32_16_2 res0.[8] res0.[10];
-  vec_interleave_low_n_lemma_uint32_16_2 res0.[9] res0.[11];
-  vec_interleave_low_n_lemma_uint32_16_2 res0.[12] res0.[14];
-  vec_interleave_low_n_lemma_uint32_16_2 res0.[13] res0.[15];
-
-  vec_interleave_high_n_lemma_uint32_16_2 res0.[0] res0.[2];
-  vec_interleave_high_n_lemma_uint32_16_2 res0.[1] res0.[3];
-  vec_interleave_high_n_lemma_uint32_16_2 res0.[4] res0.[6];
-  vec_interleave_high_n_lemma_uint32_16_2 res0.[5] res0.[7];
-  vec_interleave_high_n_lemma_uint32_16_2 res0.[8] res0.[10];
-  vec_interleave_high_n_lemma_uint32_16_2 res0.[9] res0.[11];
-  vec_interleave_high_n_lemma_uint32_16_2 res0.[12] res0.[14];
-  vec_interleave_high_n_lemma_uint32_16_2 res0.[13] res0.[15];
-
-  vec_interleave_low_lemma_uint32_16 vs0.[0] vs0.[1];
-  vec_interleave_low_lemma_uint32_16 vs0.[2] vs0.[3];
-  vec_interleave_low_lemma_uint32_16 vs0.[4] vs0.[5];
-  vec_interleave_low_lemma_uint32_16 vs0.[6] vs0.[7];
-  vec_interleave_low_lemma_uint32_16 vs0.[8] vs0.[9];
-  vec_interleave_low_lemma_uint32_16 vs0.[10] vs0.[11];
-  vec_interleave_low_lemma_uint32_16 vs0.[12] vs0.[13];
-  vec_interleave_low_lemma_uint32_16 vs0.[14] vs0.[15];
-
-  vec_interleave_high_lemma_uint32_16 vs0.[0] vs0.[1];
-  vec_interleave_high_lemma_uint32_16 vs0.[2] vs0.[3];
-  vec_interleave_high_lemma_uint32_16 vs0.[4] vs0.[5];
-  vec_interleave_high_lemma_uint32_16 vs0.[6] vs0.[7];
-  vec_interleave_high_lemma_uint32_16 vs0.[8] vs0.[9];
-  vec_interleave_high_lemma_uint32_16 vs0.[10] vs0.[11];
-  vec_interleave_high_lemma_uint32_16 vs0.[12] vs0.[13];
-  vec_interleave_high_lemma_uint32_16 vs0.[14] vs0.[15]
-#pop-options
-
-
 let transpose4x4_lemma #t vs =
   match t with
   | U32 -> Classical.forall_intro_2 (transpose4x4_lemma_uint32_ij vs)
@@ -633,9 +321,3 @@ let transpose4x4_lemma #t vs =
 let transpose8x8_lemma #t vs =
   match t with
   | U32 -> Classical.forall_intro_2 (transpose8x8_lemma_uint32_ij vs)
-  | U64 -> Classical.forall_intro_2 (transpose8x8_lemma_uint64_ij vs)
-
-
-let transpose16x16_lemma #t vs =
-  match t with
-  | U32 -> Classical.forall_intro_2 (transpose16x16_lemma_ij vs)
