lib/Lib.IntVector.Serialize.fsti
@@ -8,9 +8,9 @@ open Lib.IntVector
 module BSeq = Lib.ByteSequence
 module LSeq = Lib.Sequence
 
-#set-options "--z3rlimit 20 --max_fuel 0 --max_ifuel 0"
+#set-options "--z3rlimit 20 --fuel 0 --ifuel 0"
 
-inline_for_extraction noextract
+inline_for_extraction
 val vecs_from_bytes_le: vt:v_inttype -> w:width -> len:nat{len * (numbytes vt * w) <= max_size_t}
   -> b:lseq uint8 (len * (numbytes vt * w)) -> lseq (vec_t vt w) len
 
@@ -19,7 +19,7 @@ val index_vecs_from_bytes_le: vt:v_inttype -> w:width -> len:nat{len * (numbytes
   Lemma ((vecs_from_bytes_le vt w len b).[i] == vec_from_bytes_le vt w (LSeq.sub b (i * (numbytes vt * w)) (numbytes vt * w)))
 
 
-inline_for_extraction noextract
+inline_for_extraction
 val vecs_from_bytes_be: vt:v_inttype -> w:width -> len:nat{len * (numbytes vt * w) <= max_size_t}
   -> b:lseq uint8 (len * (numbytes vt * w)) -> lseq (vec_t vt w) len
 
@@ -27,7 +27,7 @@ val index_vecs_from_bytes_be: vt:v_inttype -> w:width -> len:nat{len * (numbytes
   -> b:lseq uint8 (len * (numbytes vt * w)) -> i:nat{i < len} ->
   Lemma ((vecs_from_bytes_be vt w len b).[i] == vec_from_bytes_be vt w (LSeq.sub b (i * (numbytes vt * w)) (numbytes vt * w)))
 
-inline_for_extraction noextract
+inline_for_extraction
 val vecs_to_bytes_le: #vt:v_inttype -> #w:width -> #len:nat{len * (numbytes vt * w) <= max_size_t}
   -> vl:lseq (vec_t vt w) len -> lseq uint8 (len * (numbytes vt * w))
 
@@ -35,7 +35,7 @@ val index_vecs_to_bytes_le: #vt:v_inttype -> #w:width -> #len:nat{len * (numbyte
   -> vl:lseq (vec_t vt w) len -> i:nat{i < len * (numbytes vt * w)} ->
   Lemma ((vecs_to_bytes_le #vt #w #len vl).[i] == (vec_to_bytes_le vl.[i / (numbytes vt * w)]).[i % (numbytes vt * w)])
 
-inline_for_extraction noextract
+inline_for_extraction
 val vecs_to_bytes_be: #vt:v_inttype -> #w:width -> #len:nat{len * (numbytes vt * w) <= max_size_t}
   -> vl:lseq (vec_t vt w) len -> lseq uint8 (len * (numbytes vt * w))
 
@@ -51,7 +51,7 @@ module B = Lib.Buffer
 module ST = FStar.HyperStack.ST
 
 
-inline_for_extraction noextract
+inline_for_extraction
 val vecs_load_le:
     #vt:v_inttype
   -> #w:width
@@ -65,7 +65,7 @@ val vecs_load_le:
       as_seq h1 o == vecs_from_bytes_le vt w (v len) (as_seq h0 i))
 
 
-inline_for_extraction noextract
+inline_for_extraction
 val vecs_load_be:
     #vt:v_inttype
   -> #w:width
@@ -79,7 +79,7 @@ val vecs_load_be:
       as_seq h1 o == vecs_from_bytes_be vt w (v len) (as_seq h0 i))
 
 
-inline_for_extraction noextract
+inline_for_extraction
 val vecs_store_le:
     #vt:v_inttype
   -> #w:width
@@ -93,7 +93,7 @@ val vecs_store_le:
       as_seq h1 o == vecs_to_bytes_le #vt #w #(v len) (as_seq h0 i))
 
 
-inline_for_extraction noextract
+inline_for_extraction
 val vecs_store_be:
     #vt:v_inttype
   -> #w:width
