lib/Lib.IntVector.fst
@@ -276,7 +276,6 @@ let vec_interleave_low_n (#t:v_inttype) (#w:width) (n:width) (x:vec_t t w) (y:ve
   | U64,4,2 -> vec256_interleave_low128 x y
   | _ -> admit()
 
-let vec_interleave_low_lemma1 #t #w v1 v2 = ()
 let vec_interleave_low_lemma2 #t v1 v2 = admit()
 let vec_interleave_low_lemma_uint32_4 v1 v2 = admit()
 let vec_interleave_low_n_lemma_uint32_4_2 v1 v2 = admit()
@@ -285,16 +284,8 @@ let vec_interleave_low_lemma_uint32_8 v1 v2 = admit()
 let vec_interleave_low_n_lemma_uint32_8_2 v1 v2 = admit()
 let vec_interleave_low_n_lemma_uint32_8_4 v1 v2 = admit()
 
-let vec_interleave_low_lemma_uint32_16 v1 v2 = admit()
-let vec_interleave_low_n_lemma_uint32_16_2 v1 v2 = admit()
-let vec_interleave_low_n_lemma_uint32_16_4 v1 v2 = admit()
-let vec_interleave_low_n_lemma_uint32_16_8 v1 v2 = admit()
-
 let vec_interleave_low_lemma_uint64_4 v1 v2 = admit()
 let vec_interleave_low_n_lemma_uint64_4_2 v1 v2 = admit()
-let vec_interleave_low_lemma_uint64_8 v1 v2 = admit()
-let vec_interleave_low_n_lemma_uint64_8_2 v1 v2 = admit()
-let vec_interleave_low_n_lemma_uint64_8_4 v1 v2 = admit()
 
 inline_for_extraction noextract
 let vec_interleave_high_ (#t:v_inttype) (#w:width) (x:vec_t t w) (y:vec_t t w) =
@@ -316,7 +307,6 @@ let vec_interleave_high_n (#t:v_inttype) (#w:width) (n:width) (x:vec_t t w) (y:v
   | U64,4,2 -> vec256_interleave_high128 x y
   | _ -> admit()
 
-let vec_interleave_high_lemma1 #t #w v1 v2 = ()
 let vec_interleave_high_lemma2 #t v1 v2 = admit()
 let vec_interleave_high_lemma_uint32_4 v1 v2 = admit()
 let vec_interleave_high_n_lemma_uint32_4_2 v1 v2 = admit()
@@ -325,16 +315,8 @@ let vec_interleave_high_lemma_uint32_8 v1 v2 = admit()
 let vec_interleave_high_n_lemma_uint32_8_2 v1 v2 = admit()
 let vec_interleave_high_n_lemma_uint32_8_4 v1 v2 = admit()
 
-let vec_interleave_high_lemma_uint32_16 v1 v2 = admit()
-let vec_interleave_high_n_lemma_uint32_16_2 v1 v2 = admit()
-let vec_interleave_high_n_lemma_uint32_16_4 v1 v2 = admit()
-let vec_interleave_high_n_lemma_uint32_16_8 v1 v2 = admit()
-
 let vec_interleave_high_lemma_uint64_4 v1 v2 = admit()
 let vec_interleave_high_n_lemma_uint64_4_2 v1 v2 = admit()
-let vec_interleave_high_lemma_uint64_8 v1 v2 = admit()
-let vec_interleave_high_n_lemma_uint64_8_2 v1 v2 = admit()
-let vec_interleave_high_n_lemma_uint64_8_4 v1 v2 = admit()
 
 let vec_shift_right_uint128_small2 v1 s = admit()
 
