lib/Lib.IntVector.fsti
@@ -70,7 +70,6 @@ val vec_get: #t:v_inttype -> #w:width
 inline_for_extraction
 val vec_add_mod: #t:v_inttype -> #w:width -> v1:vec_t t w -> v2:vec_t t w -> vec_t t w
 
-
 val vec_add_mod_lemma: #t:v_inttype -> #w:width -> v1:vec_t t w -> v2:vec_t t w -> Lemma
   (ensures (vec_v (vec_add_mod v1 v2) == map2 ( +. ) (vec_v v1) (vec_v v2)))
   [SMTPat (vec_v (vec_add_mod #t #w v1 v2))]
@@ -186,50 +185,11 @@ val vec_interleave_low_n_lemma_uint32_8_4: v1:vec_t U32 8 -> v2:vec_t U32 8 -> L
   (ensures (vec_v (vec_interleave_low_n 4 v1 v2) ==
     create8 (vec_v v1).[0] (vec_v v1).[1] (vec_v v1).[2] (vec_v v1).[3] (vec_v v2).[0] (vec_v v2).[1] (vec_v v2).[2] (vec_v v2).[3]))
 
-
-val vec_interleave_low_lemma_uint32_16: v1:vec_t U32 16 -> v2:vec_t U32 16 -> Lemma
-  (ensures (vec_v (vec_interleave_low v1 v2) ==
-    create16
-      (vec_v v1).[0] (vec_v v2).[0] (vec_v v1).[1] (vec_v v2).[1] (vec_v v1).[4] (vec_v v2).[4] (vec_v v1).[5] (vec_v v2).[5]
-      (vec_v v1).[8] (vec_v v2).[8] (vec_v v1).[9] (vec_v v2).[9] (vec_v v1).[12] (vec_v v2).[12] (vec_v v1).[13] (vec_v v2).[13]))
-
-val vec_interleave_low_n_lemma_uint32_16_2: v1:vec_t U32 16 -> v2:vec_t U32 16 -> Lemma
-  (ensures (vec_v (vec_interleave_low_n 2 v1 v2) ==
-    create16
-      (vec_v v1).[0] (vec_v v1).[1] (vec_v v2).[0] (vec_v v2).[1] (vec_v v1).[4] (vec_v v1).[5] (vec_v v2).[4] (vec_v v2).[5]
-      (vec_v v1).[8] (vec_v v1).[9] (vec_v v2).[8] (vec_v v2).[9] (vec_v v1).[12] (vec_v v1).[13] (vec_v v2).[12] (vec_v v2).[13]))
-
-val vec_interleave_low_n_lemma_uint32_16_4: v1:vec_t U32 16 -> v2:vec_t U32 16 -> Lemma
-  (ensures (vec_v (vec_interleave_low_n 4 v1 v2) ==
-    create16
-      (vec_v v1).[0] (vec_v v1).[1] (vec_v v1).[2] (vec_v v1).[3] (vec_v v2).[0] (vec_v v2).[1] (vec_v v2).[2] (vec_v v2).[3]
-      (vec_v v1).[8] (vec_v v1).[9] (vec_v v1).[10] (vec_v v1).[11] (vec_v v2).[8] (vec_v v2).[9] (vec_v v2).[10] (vec_v v2).[11]))
-
-val vec_interleave_low_n_lemma_uint32_16_8: v1:vec_t U32 16 -> v2:vec_t U32 16 -> Lemma
-  (ensures (vec_v (vec_interleave_low_n 8 v1 v2) ==
-    create16
-      (vec_v v1).[0] (vec_v v1).[1] (vec_v v1).[2] (vec_v v1).[3] (vec_v v1).[4] (vec_v v1).[5] (vec_v v1).[6] (vec_v v1).[7]
-      (vec_v v2).[0] (vec_v v2).[1] (vec_v v2).[2] (vec_v v2).[3] (vec_v v2).[4] (vec_v v2).[5] (vec_v v2).[6] (vec_v v2).[7]))
-
-
 val vec_interleave_low_lemma_uint64_4: v1:vec_t U64 4 -> v2:vec_t U64 4 -> Lemma
   (ensures (vec_v (vec_interleave_low v1 v2) == create4 (vec_v v1).[0] (vec_v v2).[0] (vec_v v1).[2] (vec_v v2).[2]))
 
 val vec_interleave_low_n_lemma_uint64_4_2: v1:vec_t U64 4 -> v2:vec_t U64 4 -> Lemma
   (ensures (vec_v (vec_interleave_low_n 2 v1 v2) == create4 (vec_v v1).[0] (vec_v v1).[1] (vec_v v2).[0] (vec_v v2).[1]))
-
-val vec_interleave_low_lemma_uint64_8: v1:vec_t U64 8 -> v2:vec_t U64 8 -> Lemma
-  (ensures (vec_v (vec_interleave_low v1 v2) ==
-    create8 (vec_v v1).[0] (vec_v v2).[0] (vec_v v1).[2] (vec_v v2).[2] (vec_v v1).[4] (vec_v v2).[4] (vec_v v1).[6] (vec_v v2).[6]))
-
-val vec_interleave_low_n_lemma_uint64_8_2: v1:vec_t U64 8 -> v2:vec_t U64 8 -> Lemma
-  (ensures (vec_v (vec_interleave_low_n 2 v1 v2) ==
-    create8 (vec_v v1).[0] (vec_v v1).[1] (vec_v v2).[0] (vec_v v2).[1] (vec_v v1).[4] (vec_v v1).[5] (vec_v v2).[4] (vec_v v2).[5]))
-
-val vec_interleave_low_n_lemma_uint64_8_4: v1:vec_t U64 8 -> v2:vec_t U64 8 -> Lemma
-  (ensures (vec_v (vec_interleave_low_n 4 v1 v2) ==
-    create8 (vec_v v1).[0] (vec_v v1).[1] (vec_v v1).[2] (vec_v v1).[3] (vec_v v2).[0] (vec_v v2).[1] (vec_v v2).[2] (vec_v v2).[3]))
-
 
 inline_for_extraction
 val vec_interleave_high_n: #t:v_inttype -> #w:width -> n:width{w % n == 0} -> vec_t t w -> vec_t t w -> vec_t t w
@@ -241,13 +201,11 @@ let vec_interleave_high (#t:v_inttype) (#w:width) (v1:vec_t t w) (v2:vec_t t w) 
 val vec_interleave_high_lemma2: #t:v_inttype -> v1:vec_t t 2 -> v2:vec_t t 2 -> Lemma
   (ensures (vec_v (vec_interleave_high v1 v2) == create2 (vec_v v1).[1] (vec_v v2).[1]))
 
-
 val vec_interleave_high_lemma_uint32_4: v1:vec_t U32 4 -> v2:vec_t U32 4 -> Lemma
   (ensures (vec_v (vec_interleave_high v1 v2) == create4 (vec_v v1).[2] (vec_v v2).[2] (vec_v v1).[3] (vec_v v2).[3]))
 
 val vec_interleave_high_n_lemma_uint32_4_2: v1:vec_t U32 4 -> v2:vec_t U32 4 -> Lemma
   (ensures (vec_v (vec_interleave_high_n 2 v1 v2) == create4 (vec_v v1).[2] (vec_v v1).[3] (vec_v v2).[2] (vec_v v2).[3]))
-
 
 val vec_interleave_high_lemma_uint32_8: v1:vec_t U32 8 -> v2:vec_t U32 8 -> Lemma
   (ensures (vec_v (vec_interleave_high v1 v2) ==
@@ -261,49 +219,11 @@ val vec_interleave_high_n_lemma_uint32_8_4: v1:vec_t U32 8 -> v2:vec_t U32 8 -> 
   (ensures (vec_v (vec_interleave_high_n 4 v1 v2) ==
     create8 (vec_v v1).[4] (vec_v v1).[5] (vec_v v1).[6] (vec_v v1).[7] (vec_v v2).[4] (vec_v v2).[5] (vec_v v2).[6] (vec_v v2).[7]))
 
-
-val vec_interleave_high_lemma_uint32_16: v1:vec_t U32 16 -> v2:vec_t U32 16 -> Lemma
-  (ensures (vec_v (vec_interleave_high v1 v2) ==
-    create16
-      (vec_v v1).[2] (vec_v v2).[2] (vec_v v1).[3] (vec_v v2).[3] (vec_v v1).[6] (vec_v v2).[6] (vec_v v1).[7] (vec_v v2).[7]
-      (vec_v v1).[10] (vec_v v2).[10] (vec_v v1).[11] (vec_v v2).[11] (vec_v v1).[14] (vec_v v2).[14] (vec_v v1).[15] (vec_v v2).[15]))
-
-val vec_interleave_high_n_lemma_uint32_16_2: v1:vec_t U32 16 -> v2:vec_t U32 16 -> Lemma
-  (ensures (vec_v (vec_interleave_high_n 2 v1 v2) ==
-    create16
-      (vec_v v1).[2] (vec_v v1).[3] (vec_v v2).[2] (vec_v v2).[3] (vec_v v1).[6] (vec_v v1).[7] (vec_v v2).[6] (vec_v v2).[7]
-      (vec_v v1).[10] (vec_v v1).[11] (vec_v v2).[10] (vec_v v2).[11] (vec_v v1).[14] (vec_v v1).[15] (vec_v v2).[14] (vec_v v2).[15]))
-
-val vec_interleave_high_n_lemma_uint32_16_4: v1:vec_t U32 16 -> v2:vec_t U32 16 -> Lemma
-  (ensures (vec_v (vec_interleave_high_n 4 v1 v2) ==
-    create16
-      (vec_v v1).[4] (vec_v v1).[5] (vec_v v1).[6] (vec_v v1).[7] (vec_v v2).[4] (vec_v v2).[5] (vec_v v2).[6] (vec_v v2).[7]
-      (vec_v v1).[12] (vec_v v1).[13] (vec_v v1).[14] (vec_v v1).[15] (vec_v v2).[12] (vec_v v2).[13] (vec_v v2).[14] (vec_v v2).[15]))
-
-val vec_interleave_high_n_lemma_uint32_16_8: v1:vec_t U32 16 -> v2:vec_t U32 16 -> Lemma
-  (ensures (vec_v (vec_interleave_high_n 8 v1 v2) ==
-    create16
-      (vec_v v1).[8] (vec_v v1).[9] (vec_v v1).[10] (vec_v v1).[11] (vec_v v1).[12] (vec_v v1).[13] (vec_v v1).[14] (vec_v v1).[15]
-      (vec_v v2).[8] (vec_v v2).[9] (vec_v v2).[10] (vec_v v2).[11] (vec_v v2).[12] (vec_v v2).[13] (vec_v v2).[14] (vec_v v2).[15]))
-
-
 val vec_interleave_high_lemma_uint64_4: v1:vec_t U64 4 -> v2:vec_t U64 4 -> Lemma
   (ensures (vec_v (vec_interleave_high v1 v2) == create4 (vec_v v1).[1] (vec_v v2).[1] (vec_v v1).[3] (vec_v v2).[3]))
 
 val vec_interleave_high_n_lemma_uint64_4_2: v1:vec_t U64 4 -> v2:vec_t U64 4 -> Lemma
   (ensures (vec_v (vec_interleave_high_n 2 v1 v2) == create4 (vec_v v1).[2] (vec_v v1).[3] (vec_v v2).[2] (vec_v v2).[3]))
-
-val vec_interleave_high_lemma_uint64_8: v1:vec_t U64 8 -> v2:vec_t U64 8 -> Lemma
-  (ensures (vec_v (vec_interleave_high v1 v2) ==
-    create8 (vec_v v1).[1] (vec_v v2).[1] (vec_v v1).[3] (vec_v v2).[3] (vec_v v1).[5] (vec_v v2).[5] (vec_v v1).[7] (vec_v v2).[7]))
-
-val vec_interleave_high_n_lemma_uint64_8_2: v1:vec_t U64 8 -> v2:vec_t U64 8 -> Lemma
-  (ensures (vec_v (vec_interleave_high_n 2 v1 v2) ==
-    create8 (vec_v v1).[2] (vec_v v1).[3] (vec_v v2).[2] (vec_v v2).[3] (vec_v v1).[6] (vec_v v1).[7] (vec_v v2).[6] (vec_v v2).[7]))
-
-val vec_interleave_high_n_lemma_uint64_8_4: v1:vec_t U64 8 -> v2:vec_t U64 8 -> Lemma
-  (ensures (vec_v (vec_interleave_high_n 4 v1 v2) ==
-    create8 (vec_v v1).[4] (vec_v v1).[5] (vec_v v1).[6] (vec_v v1).[7] (vec_v v2).[4] (vec_v v2).[5] (vec_v v2).[6] (vec_v v2).[7]))
 
 val vec_shift_right_uint128_small2: v1:vec_t U64 4 -> s:shiftval U128{uint_v s % 8 == 0 /\ 0 < uint_v s /\ uint_v s < 64} -> Lemma
   (let v2 = cast U64 4 (vec_shift_right (cast U128 2 v1) s) in
@@ -326,7 +246,6 @@ val vec_rotate_right_lanes4_lemma: #t:v_inttype -> v1:vec_t t 4 -> s:size_t{v s 
   Lemma (ensures (vec_v (vec_rotate_right_lanes v1 s) ==
                   create4 (vec_v v1).[(v s) % 4] (vec_v v1).[(v s + 1) % 4] (vec_v v1).[(v s + 2) % 4] (vec_v v1).[(v s + 3) % 4]))
 	[SMTPat (vec_v (vec_rotate_right_lanes #t v1 s))]
-
 
 inline_for_extraction
 val vec_rotate_left_lanes: #t:v_inttype -> #w:width
