lib/Lib.NTuple.fsti
@@ -3,19 +3,19 @@ module Lib.NTuple
 open FStar.Mul
 open Lib.IntTypes
 
-#set-options "--z3rlimit 15 --max_ifuel 0 --max_fuel 0"
+#set-options "--z3rlimit 15 --ifuel 0 --fuel 0"
 
 /// Fixed and bounded length sequences, implemented using tuples
 
 inline_for_extraction
 let flen = size_pos
 
-inline_for_extraction noextract
+inline_for_extraction
 let rec ntuple_ (a:Type0) (len:flen) =
   if len = 1 then a
   else a & ntuple_ a (len-1)
 
-inline_for_extraction noextract
+inline_for_extraction
 let ntuple (a:Type0) (len:flen) = normalize_term (ntuple_ a len)
 
 inline_for_extraction
@@ -24,21 +24,17 @@ val fst (#a:Type0) (#len:flen) (s:ntuple a len) : a
 inline_for_extraction
 val rest (#a:Type0) (#len:flen{len > 1}) (s:ntuple a len) : ntuple a (len - 1)
 
-inline_for_extraction noextract
+inline_for_extraction
 val index (#a:Type0) (#len:flen) (s:ntuple a len) (i:nat{i < len}) : a
 
 val index_fst_lemma (#a:Type0) (#len:flen) (s:ntuple a len) :
   Lemma (fst s == index s 0)
   [SMTPat (fst s)]
 
-// val index_rest_lemma (#a:Type0) (#len:flen{len > 1}) (s:ntuple a len) (i:nat{i < len - 1}) :
-//   Lemma (index s (i + 1) == index (rest s) i)
-//   [SMTPat (index (rest s) i)]
-
-inline_for_extraction noextract
+inline_for_extraction
 val createi (#a:Type0) (len:flen) (f:(i:nat{i < len} -> a)) : ntuple a len
 
-inline_for_extraction noextract
+inline_for_extraction
 val gcreatei (#a:Type0) (len:flen) (f:(i:nat{i < len} -> GTot a)) : GTot (ntuple a len)
 
 val createi_lemma (#a:Type0) (len:flen) (f:(i:nat{i < len} -> a)) (i:nat{i < len}) :
@@ -49,20 +45,23 @@ val gcreatei_lemma (#a:Type0) (len:flen) (f:(i:nat{i < len} -> GTot a)) (i:nat{i
   Lemma (index (gcreatei #a len f) i == f i)
   [SMTPat (index (gcreatei #a len f) i)]
 
-inline_for_extraction noextract
+inline_for_extraction
 val to_lseq (#a:Type0) (#len:flen) (l:ntuple a len) : Lib.Sequence.lseq a len
 
-inline_for_extraction noextract
+val to_lseq_index (#a:Type0) (#len:flen) (l:ntuple a len) (i:nat{i < len}) :
+  Lemma (index l i == Lib.Sequence.index (to_lseq l) i)
+
+inline_for_extraction
 val from_lseq (#a:Type0) (#len:flen) (s:Lib.Sequence.lseq a len) : ntuple a len
 
-inline_for_extraction noextract
+inline_for_extraction
 val create (#a:Type0) (len:flen) (init:a) : ntuple a len
 
 val create_lemma (#a:Type0) (len:flen) (init:a) (i:nat{i < len}) :
   Lemma (index (create #a len init) i == init)
   [SMTPat (index (create #a len init) i)]
 
-inline_for_extraction noextract
+inline_for_extraction
 val concat (#a:Type0) (#len0:flen) (#len1:flen{len0 + len1 <= max_size_t})
 	   (s0:ntuple a len0) (s1:ntuple a len1) : ntuple a (len0 + len1)
 
@@ -74,7 +73,7 @@ val concat_lemma (#a:Type0) (#len0:flen) (#len1:flen) (s0:ntuple a len0) (s1:ntu
             (i >= len0 ==> index (concat s0 s1) i == index s1 (i-len0))))
   [SMTPat (index (concat #a #len0 #len1 s0 s1) i)]
 
-inline_for_extraction noextract
+inline_for_extraction
 val equal (#a:Type) (#len:flen) (s1:ntuple a len) (s2:ntuple a len) : Type0
 
 val eq_intro: #a:Type -> #len:flen -> s1:ntuple a len -> s2:ntuple a len ->
@@ -91,21 +90,21 @@ val eq_elim: #a:Type -> #len:flen -> s1:ntuple a len -> s2:ntuple a len ->
 
 (** Updating an element of a fixed-length Sequence *)
 
-inline_for_extraction noextract
+inline_for_extraction
 val upd: #a:Type -> #len:flen -> s:ntuple a len -> i:nat{i < len} -> x:a -> ntuple a len
 
 val upd_lemma (#a:Type0) (#len:flen) (s:ntuple a len) (i:nat{i < len}) (x:a) (j:nat{j < len}) :
   Lemma (index (upd #a #len s i x) j == (if i = j then x else index s j))
   [SMTPat (index (upd #a #len s i x) j)]
 
-inline_for_extraction noextract
+inline_for_extraction
 val sub (#a:Type) (#len:flen) (s:ntuple a len) (start:nat) (n:flen{start + n <= len}) : ntuple a n
 
 val index_sub_lemma (#a:Type) (#len:flen) (s:ntuple a len) (start:nat) (n:flen{start + n <= len}) (i:nat{i < n}) :
   Lemma (index (sub #a #len s start n) i == index s (start + i))
   [SMTPat (index (sub #a #len s start n) i)]
 
-inline_for_extraction noextract
+inline_for_extraction
 val update_sub (#a:Type) (#len:flen) (s:ntuple a len) (start:nat) (n:flen{start + n <= len}) (x:ntuple a n) : ntuple a len
 
 val index_update_sub_lemma (#a:Type) (#len:flen) (s:ntuple a len) (start:nat) (n:flen{start + n <= len}) (x:ntuple a n) (i:nat{i < n}) :
@@ -113,42 +112,42 @@ val index_update_sub_lemma (#a:Type) (#len:flen) (s:ntuple a len) (start:nat) (n
   (index (update_sub #a #len s start n x) i == (if i >= start && i < start + n then index x (i - start) else index s i))
   [SMTPat (index (update_sub #a #len s start n x) i)]
 
-inline_for_extraction noextract
+inline_for_extraction
 val mapi (#a:Type) (#b:Type) (#len:flen) (f:(i:nat{i < len} -> a -> b)) (s:ntuple a len) : ntuple b len
 
 val index_mapi_lemma (#a:Type) (#b:Type) (#len:flen) (f:(i:nat{i < len} -> a -> b)) (s:ntuple a len) (i:nat{i < len}) :
   Lemma (index (mapi #a #b #len f s) i == f i (index s i))
   [SMTPat (index (mapi #a #b #len f s) i)]
 
-inline_for_extraction noextract
+inline_for_extraction
 val gmapi (#a:Type) (#b:Type) (#len:flen) (f:(i:nat{i < len} -> a -> GTot b)) (s:ntuple a len) : GTot (ntuple b len)
 
 val index_gmapi_lemma (#a:Type) (#b:Type) (#len:flen) (f:(i:nat{i < len} -> a -> GTot b)) (s:ntuple a len) (i:nat{i < len}) :
   Lemma (index (gmapi #a #b #len f s) i == f i (index s i))
   [SMTPat (index (gmapi #a #b #len f s) i)]
 
-inline_for_extraction noextract
+inline_for_extraction
 val map (#a:Type) (#b:Type) (#len:flen) (f:a -> b) (s:ntuple a len) : ntuple b len
 
 val index_map_lemma (#a:Type) (#b:Type) (#len:flen) (f:(a -> b)) (s:ntuple a len) (i:nat{i < len}) :
   Lemma (index (map #a #b #len f s) i == f (index s i))
   [SMTPat (index (map #a #b #len f s) i)]
 
-inline_for_extraction noextract
+inline_for_extraction
 val gmap (#a:Type) (#b:Type) (#len:flen) (f:a -> GTot b) (s:ntuple a len) : GTot (ntuple b len)
 
 val index_gmap_lemma (#a:Type) (#b:Type) (#len:flen) (f:(a -> GTot b)) (s:ntuple a len) (i:nat{i < len}) :
   Lemma (index (gmap #a #b #len f s) i == f (index s i))
   [SMTPat (index (gmap #a #b #len f s) i)]
 
-inline_for_extraction noextract
+inline_for_extraction
 val map2i (#a:Type) (#b:Type) (#c:Type) (#len:flen) (f:(i:nat{i < len} -> a -> b -> c)) (s1:ntuple a len)  (s2:ntuple b len) : ntuple c len
 
 val index_map2i_lemma (#a:Type) (#b:Type) (#c:Type) (#len:flen) (f:(i:nat{i < len} -> a -> b -> c)) (s1:ntuple a len)  (s2:ntuple b len) (i:nat{i < len}) :
   Lemma (index (map2i #a #b #c #len f s1 s2) i == f i (index s1 i) (index s2 i))
   [SMTPat (index (map2i #a #b #c #len f s1 s2) i)]
 
-inline_for_extraction noextract
+inline_for_extraction
 val map2 (#a:Type) (#b:Type) (#c:Type) (#len:flen) (f:(a -> b -> c)) (s1:ntuple a len)  (s2:ntuple b len) : ntuple c len
 
 val index_map2_lemma (#a:Type) (#b:Type) (#c:Type) (#len:flen) (f:a -> b -> c) (s1:ntuple a len)  (s2:ntuple b len) (i:nat{i < len}) :
@@ -159,7 +158,7 @@ unfold let op_Lens_Access #a #len = index #a #len
 unfold let op_Lens_Assignment #a #len = upd #a #len
 
 (* The following conversions are tedious, but are needed to aid KreMLin in extracting ntuples correctly *)
-inline_for_extraction noextract
+inline_for_extraction
 let ntup1 #a (#l:flen{l = 1}) (t:a) : ntuple a l =
   assert (ntuple a l == ntuple a 1);
   t <: ntuple a 1
@@ -168,7 +167,7 @@ val ntup1_lemma (#a:Type0) (#l:flen{l == 1}) (t:a):
   Lemma (let x0 = t in let t = ntup1 #a #l t in x0 == t.(|0|))
   [SMTPat (ntup1 #a #l t)]
 
-inline_for_extraction noextract
+inline_for_extraction
 let tup1 #a (#l:flen{l = 1}) (t:ntuple a l) : a =
   assert (ntuple a l == ntuple a 1);
   t <: ntuple a 1
@@ -177,9 +176,9 @@ val tup1_lemma (#a:Type0) (#l:flen{l == 1}) (t:ntuple a l):
   Lemma (let x0 = tup1 t in x0 == t.(|0|))
   [SMTPat (tup1 #a #l t)]
 
-#set-options "--max_fuel 4"
+#set-options "--fuel 4"
 
-inline_for_extraction noextract
+inline_for_extraction
 let ntup4 #a (#l:flen{l = 4}) (t:a & (a & (a & a))) : ntuple a l =
   assert (ntuple a l == ntuple a 4);
   (t <: ntuple a 4)
@@ -188,13 +187,11 @@ val ntup4_lemma (#a:Type0) (#l:flen{l == 4}) (t:a & (a & (a & a))) :
   Lemma
    (let (x0,(x1,(x2,x3))) = t in
     let t = ntup4 #a #l t in
-    x0 == t.(|0|) /\
-    x1 == t.(|1|) /\
-    x2 == t.(|2|) /\
-    x3 == t.(|3|))
+    x0 == t.(|0|) /\ x1 == t.(|1|) /\
+    x2 == t.(|2|) /\ x3 == t.(|3|))
   [SMTPat (ntup4 #a #l t)]
 
-inline_for_extraction noextract
+inline_for_extraction
 let tup4 #a (#l:flen{l = 4}) (t:ntuple a l) : (a & (a & (a & a))) =
   assert (ntuple a l == ntuple a 4);
   (t <: ntuple a 4)
@@ -202,15 +199,13 @@ let tup4 #a (#l:flen{l = 4}) (t:ntuple a l) : (a & (a & (a & a))) =
 val tup4_lemma (#a:Type0) (#l:flen{l = 4}) (t:ntuple a l) :
   Lemma
    (let (x0,(x1,(x2,x3))) = tup4 t in
-    x0 == t.(|0|) /\
-    x1 == t.(|1|) /\
-    x2 == t.(|2|) /\
-    x3 == t.(|3|))
+    x0 == t.(|0|) /\ x1 == t.(|1|) /\
+    x2 == t.(|2|) /\ x3 == t.(|3|))
   [SMTPat (tup4 t)]
 
-#set-options "--max_fuel 8 --max_ifuel 8"
+#set-options "--fuel 8"
 
-inline_for_extraction noextract
+inline_for_extraction
 let ntup8 #a (#l:flen{l = 8}) (t:a & (a & (a & (a & (a & (a & (a & a))))))) : ntuple a l =
   assert (ntuple a l == ntuple a 8);
   (t <: ntuple a 8)
@@ -219,17 +214,13 @@ val ntup8_lemma (#a:Type0) (#l:flen{l == 8}) (t:a & (a & (a & (a & (a & (a & (a 
   Lemma
    (let (x0,(x1,(x2,(x3,(x4,(x5,(x6,x7))))))) = t in
     let t = ntup8 #a #l t in
-    x0 == t.(|0|) /\
-    x1 == t.(|1|) /\
-    x2 == t.(|2|) /\
-    x3 == t.(|3|) /\
-    x4 == t.(|4|) /\
-    x5 == t.(|5|) /\
-    x6 == t.(|6|) /\
-    x7 == t.(|7|))
+    x0 == t.(|0|) /\ x1 == t.(|1|) /\
+    x2 == t.(|2|) /\ x3 == t.(|3|) /\
+    x4 == t.(|4|) /\ x5 == t.(|5|) /\
+    x6 == t.(|6|) /\ x7 == t.(|7|))
   [SMTPat (ntup8 #a #l t)]
 
-inline_for_extraction noextract
+inline_for_extraction
 let tup8 #a (#l:flen{l = 8}) (t:ntuple a l) : (a & (a & (a & (a & (a & (a & (a & a))))))) =
   assert (ntuple a l == ntuple a 8);
   (t <: ntuple a 8)
@@ -237,12 +228,8 @@ let tup8 #a (#l:flen{l = 8}) (t:ntuple a l) : (a & (a & (a & (a & (a & (a & (a &
 val tup8_lemma (#a:Type0) (#l:flen{l = 8}) (t:ntuple a l) :
   Lemma
    (let (x0,(x1,(x2,(x3,(x4,(x5,(x6,x7))))))) = tup8 t in
-    x0 == t.(|0|) /\
-    x1 == t.(|1|) /\
-    x2 == t.(|2|) /\
-    x3 == t.(|3|) /\
-    x4 == t.(|4|) /\
-    x5 == t.(|5|) /\
-    x6 == t.(|6|) /\
-    x7 == t.(|7|))
+    x0 == t.(|0|) /\ x1 == t.(|1|) /\
+    x2 == t.(|2|) /\ x3 == t.(|3|) /\
+    x4 == t.(|4|) /\ x5 == t.(|5|) /\
+    x6 == t.(|6|) /\ x7 == t.(|7|))
   [SMTPat (tup8 t)]
